\section{Яўны метад Эйлера}
\subsection*{Ураўненне}
\begin{equation}
    y_{n+1} = y_n + hf_n, \hspace{10pt} h = \frac{x_1-x_0}{N}, \hspace{10pt} n = \overline{0, N-1}. \\
\end{equation}

{\small
\begin{verbatim}
def euler_explicit():
    yi = [u0]
    for i in range(1, len(grid)):
        x = grid[i-1]
        step = grid[i] - grid[i-1]
        yi.append( yi[-1] + step*f(x,yi[-1]) )
    return yi
\end{verbatim}
}

{\small
\begin{verbatim}
Explicit Euler:
y(0.0) = -1.0
y(0.1) = -0.9
y(0.2) = -0.800516158585
y(0.3) = -0.702589328265
y(0.4) = -0.607236282379
y(0.5) = -0.51543831245
y(0.6) = -0.428130795736
y(0.7) = -0.346193682081
y(0.8) = -0.270442842279
y(0.9) = -0.201622227856
y(1.0) = -0.140396807646
\end{verbatim}
}

\subsection*{Сістэма}
\begin{equation}
	\begin{cases}
y_{n+1} = y_n + hf_n, \\
z_{n+1} = z_n + hg_n, \hspace{10pt} h = \frac{x_1-x_0}{N}, \hspace{10pt} n = \overline{0, N-1}.
	\end{cases}
\end{equation}

{\small
\begin{verbatim}
def euler_explicit_system():
    yi = [y0]
    zi = [z0]
    for i in range(1, len(grid)):
        step = grid[i] - grid[i-1]
        yi.append(yi[i-1] + step * f(grid[i-1], yi[i-1], zi[i-1]))
        zi.append(zi[i-1] + step * g(grid[i-1], yi[i-1], zi[i-1]))
    return (yi, zi)
\end{verbatim}
}

{\small
\begin{verbatim}
Explicit Euler for system:
Y:
y(0.0) = 0.5
y(0.05) = 0.514325239843
y(0.1) = 0.531409062083
y(0.15) = 0.551334821493
y(0.2) = 0.574239609375
y(0.25) = 0.600311215312
y(0.3) = 0.629780591884
y(0.35) = 0.662909402276
y(0.4) = 0.699973080276
y(0.45) = 0.741241007894
y(0.5) = 0.786956675174
Z:
z(0.0) = 1.0
z(0.05) = 1.075
z(0.1) = 1.15520304523
z(0.15) = 1.24120275662
z(0.2) = 1.33365990299
z(0.25) = 1.43331801104
z(0.3) = 1.54102126711
z(0.35) = 1.65773468986
z(0.4) = 1.78456631192
z(0.45) = 1.92279085882
z(0.5) = 2.07387422494
\end{verbatim}
}
